serialize string

src/cbor/raw/pulse/everparse/CBOR.Pulse.Raw.Serialize.fst
@@ -76,12 +76,39 @@ assume val l2r_write_nlist_as_array
   (p: perm)
 : l2r_writer (nlist_match_array vmatch (SZ.v n) p) (LowParse.Spec.VCList.serialize_nlist (SZ.v n) s)
 
-assume val ser_body_for_array
-  (f: (p: perm) -> LP.l2r_writer (cbor_match p) serialize_raw_data_item)
+let cbor_match_with_perm
+  (x: with_perm cbor_raw)
+  (y: raw_data_item)
+: Tot slprop
+= cbor_match x.p x.v y
+
+module Trade = Pulse.Lib.Trade.Util
+
+```pulse
+ghost
+fn cbor_match_with_perm_lens
   (p: perm)
-  (c: cbor_raw { CBOR_Case_Array? c })
+: vmatch_lens #_ #_ #_ (cbor_match p) cbor_match_with_perm
+=
+  (x: cbor_raw)
+  (y: raw_data_item)
+{
+  let res : with_perm cbor_raw = {
+    v = x;
+    p = p;
+  };
+  Trade.rewrite_with_trade
+    (cbor_match p x y)
+    (cbor_match_with_perm res y);
+  res
+}
+```
+
+assume val ser_body_for_array
+  (f: LP.l2r_writer cbor_match_with_perm serialize_raw_data_item)
+  (c: with_perm cbor_raw { CBOR_Case_Array? c.v })
   (r: Ghost.erased raw_data_item)
-: LP.l2r_writer_for (cbor_match p) serialize_raw_data_item c r
+: LP.l2r_writer_for cbor_match_with_perm serialize_raw_data_item c r
 
 ```pulse
 fn cbor_raw_get_header
@@ -125,6 +152,24 @@ ensures
 }
 ```
 
+```pulse
+fn cbor_raw_with_perm_get_header
+  (xl: with_perm cbor_raw)
+  (xh: erased raw_data_item)
+requires
+      (cbor_match_with_perm xl xh)
+returns res: header
+ensures
+          cbor_match_with_perm xl xh **
+          pure (res == get_raw_data_item_header xh)
+{
+  unfold (cbor_match_with_perm xl xh);
+  let res = cbor_raw_get_header xl.p xl.v xh;
+  fold (cbor_match_with_perm xl xh);
+  res
+}
+```
+
 let synth_raw_data_item_recip_synth_raw_data_item
   (x: _)
 : Lemma
@@ -134,31 +179,29 @@ let synth_raw_data_item_recip_synth_raw_data_item
 inline_for_extraction
 ```pulse
 fn cbor_raw_get_header'
-  (p: perm)
-  (xl: cbor_raw)
+  (xl: with_perm cbor_raw)
   (xh: erased (dtuple2 header content))
 requires
-      (LP.vmatch_synth (cbor_match p) synth_raw_data_item xl (reveal xh))
+      (LP.vmatch_synth (cbor_match_with_perm) synth_raw_data_item xl (reveal xh))
 returns res: header
 ensures
-          LP.vmatch_synth (cbor_match p) synth_raw_data_item xl (reveal xh) **
+          LP.vmatch_synth (cbor_match_with_perm) synth_raw_data_item xl (reveal xh) **
           pure (res == dfst (reveal xh))
 {
   synth_raw_data_item_recip_synth_raw_data_item xh;
-  unfold (LP.vmatch_synth (cbor_match p) synth_raw_data_item xl (reveal xh));
-  let res = cbor_raw_get_header p xl _;
-  fold (LP.vmatch_synth (cbor_match p) synth_raw_data_item xl (reveal xh));
+  unfold (LP.vmatch_synth (cbor_match_with_perm) synth_raw_data_item xl (reveal xh));
+  let res = cbor_raw_with_perm_get_header xl _;
+  fold (LP.vmatch_synth (cbor_match_with_perm) synth_raw_data_item xl (reveal xh));
   res
 }
 ```
 
 let match_cbor_payload
-  (p: perm)
   (xh1: header)
 =
         (LP.vmatch_dep_proj2
             (LP.vmatch_synth
-                (cbor_match p)
+                (cbor_match_with_perm)
                 synth_raw_data_item
             )
             xh1
@@ -166,35 +209,30 @@ let match_cbor_payload
 
 module U64 = FStar.UInt64
 
-#push-options "--print_implicits"
-
-module Trade = Pulse.Lib.Trade.Util
-
 ```pulse
 ghost
 fn ser_payload_string_lens_aux
-  (p: perm)
   (xh1: header)
   (sq: squash (let b = get_header_initial_byte xh1 in b.major_type = cbor_major_type_byte_string || b.major_type = cbor_major_type_text_string))
-  (xl: cbor_raw)
+  (xl: with_perm cbor_raw)
   (xh: content xh1)
 requires
   (vmatch_ext
       (Seq.Properties.lseq byte
                   (U64.v (argument_as_uint64 (get_header_initial_byte xh1)
                           (get_header_long_argument xh1))))
-      (match_cbor_payload p xh1) xl xh
+      (match_cbor_payload xh1) xl xh
   )
 returns xh': Ghost.erased raw_data_item
 ensures
-  (cbor_match p xl xh' **
+  (cbor_match_with_perm xl xh' **
     Trade.trade
-      (cbor_match p xl xh')
+      (cbor_match_with_perm xl xh')
       (vmatch_ext
         (Seq.Properties.lseq byte
           (U64.v (argument_as_uint64 (get_header_initial_byte xh1)
             (get_header_long_argument xh1))))
-        (match_cbor_payload p xh1) xl xh
+        (match_cbor_payload xh1) xl xh
       ) **
       pure (synth_raw_data_item_recip xh' == (| xh1, xh |))
   )
@@ -210,22 +248,24 @@ fn pts_to_seqbytes_intro
   (p: perm)
   (s: S.slice byte)
   (v: bytes)
+  (res: with_perm (S.slice byte))
 requires
-  S.pts_to s #p v ** pure (Seq.length v == n)
-returns v': Seq.lseq byte n
+  S.pts_to s #p v ** pure (Seq.length v == n /\ res.v == s /\ res.p == p)
+returns v': Ghost.erased (Seq.lseq byte n)
 ensures
-  LowParse.Pulse.SeqBytes.pts_to_seqbytes n p s v' **
+  LowParse.Pulse.SeqBytes.pts_to_seqbytes n res v' **
   Trade.trade
-    (LowParse.Pulse.SeqBytes.pts_to_seqbytes n p s v')
-    (S.pts_to s #p v)
+    (LowParse.Pulse.SeqBytes.pts_to_seqbytes n res v')
+    (S.pts_to s #p v) **
+  pure (v == Ghost.reveal v')
 {
   let v' : Seq.lseq byte n = v;
-  fold (LowParse.Pulse.SeqBytes.pts_to_seqbytes n p s v');
+  fold (LowParse.Pulse.SeqBytes.pts_to_seqbytes n res v');
   ghost fn aux (_: unit)
-    requires emp ** LowParse.Pulse.SeqBytes.pts_to_seqbytes n p s v'
+    requires emp ** LowParse.Pulse.SeqBytes.pts_to_seqbytes n res v'
     ensures S.pts_to s #p v
   {
-    unfold (LowParse.Pulse.SeqBytes.pts_to_seqbytes n p s v')
+    unfold (LowParse.Pulse.SeqBytes.pts_to_seqbytes n res v')
   };
   Trade.intro _ _ _ aux;
   v'
@@ -235,42 +275,49 @@ ensures
 inline_for_extraction
 ```pulse
 fn ser_payload_string_lens
-  (p: perm)
   (xh1: header)
   (sq: squash (let b = get_header_initial_byte xh1 in b.major_type = cbor_major_type_byte_string || b.major_type = cbor_major_type_text_string))
 : 
-vmatch_lens #cbor_raw
-  #(S.slice byte)
-  #(Seq.Properties.lseq byte
-              (U64.v (argument_as_uint64 (get_header_initial_byte xh1)
-                      (get_header_long_argument xh1))))
+vmatch_lens #_ #_ #_
   (vmatch_ext
       (Seq.Properties.lseq byte
                   (U64.v (argument_as_uint64 (get_header_initial_byte xh1)
                           (get_header_long_argument xh1))))
-      (match_cbor_payload p xh1))
+      (match_cbor_payload xh1))
   (LowParse.Pulse.SeqBytes.pts_to_seqbytes
               (U64.v (argument_as_uint64 (get_header_initial_byte xh1)
                       (get_header_long_argument xh1)))
-      p)
+  )
 = (x1': _)
   (x: _)
 {
-  let xh' = ser_payload_string_lens_aux p xh1 sq x1' x;
-  let res = cbor_match_string_elim_payload x1';
-  Trade.trans _ (cbor_match p x1' xh') _;
-  S.pts_to_len res;
-  pts_to_seqbytes_intro
+  let xh' = ser_payload_string_lens_aux xh1 sq x1' x;
+  Trade.rewrite_with_trade
+    (cbor_match_with_perm x1' xh')
+    (cbor_match x1'.p x1'.v xh');
+  Trade.trans
+    (cbor_match x1'.p x1'.v xh')
+    _ _;
+  let s = cbor_match_string_elim_payload x1'.v;
+  Trade.trans _ (cbor_match _ x1'.v xh') _;
+  S.pts_to_len s;
+  with p' . assert (S.pts_to s #p' x);
+  let res : with_perm (S.slice byte) = {
+    v = s;
+    p = p';
+  };
+  let x' = pts_to_seqbytes_intro
     (U64.v (argument_as_uint64 (get_header_initial_byte xh1)
                           (get_header_long_argument xh1)))
-    p
-    res
-    _;
+    _
+    s
+    x
+    res;
   Trade.trans
     (LowParse.Pulse.SeqBytes.pts_to_seqbytes
               (U64.v (argument_as_uint64 (get_header_initial_byte xh1)
                       (get_header_long_argument xh1)))
-      p res _)
+      res x')
     _ _;
   res
 }
@@ -278,36 +325,32 @@ vmatch_lens #cbor_raw
 
 inline_for_extraction
 let ser_payload_string
-  (p: perm)
   (xh1: header)
   (sq: squash (let b = get_header_initial_byte xh1 in b.major_type = cbor_major_type_byte_string || b.major_type = cbor_major_type_text_string))
-: l2r_writer (match_cbor_payload p xh1) (serialize_content xh1)
+: l2r_writer (match_cbor_payload xh1) (serialize_content xh1)
 = l2r_writer_ext_gen
     (l2r_writer_lens
-      (ser_payload_string_lens p xh1 sq)
+      (ser_payload_string_lens xh1 sq)
       (LowParse.Pulse.SeqBytes.l2r_write_lseq_bytes_copy
         (U64.v (argument_as_uint64 (get_header_initial_byte xh1) (get_header_long_argument xh1)))
-        p
       )
     )
     (serialize_content xh1)
 
 inline_for_extraction
 let ser_payload
-  (f: ((p: perm) -> l2r_writer (cbor_match p) serialize_raw_data_item))
-  (p: perm)
+  (f: l2r_writer (cbor_match_with_perm) serialize_raw_data_item)
   (xh1: header)
-: l2r_writer (match_cbor_payload p xh1) (serialize_content xh1)
+: l2r_writer (match_cbor_payload xh1) (serialize_content xh1)
 = l2r_writer_ifthenelse _ _
     (let b = get_header_initial_byte xh1 in b.major_type = cbor_major_type_byte_string || b.major_type = cbor_major_type_text_string)
-    (ser_payload_string p xh1)
+    (ser_payload_string xh1)
     (magic ())
 
 inline_for_extraction
 let ser_body
-  (f: (p: perm) -> LP.l2r_writer (cbor_match p) serialize_raw_data_item)
-  (p: perm)
-: LP.l2r_writer (cbor_match p) serialize_raw_data_item
+  (f: LP.l2r_writer (cbor_match_with_perm) serialize_raw_data_item)
+: LP.l2r_writer (cbor_match_with_perm) serialize_raw_data_item
 = LP.l2r_writer_ext #_ #_ #_ #_ #_ #serialize_raw_data_item_aux
     (LP.l2r_write_synth_recip
       _
@@ -315,29 +358,27 @@ let ser_body
       synth_raw_data_item_recip
       (LP.l2r_write_dtuple2_recip_explicit_header
         write_header
-        (cbor_raw_get_header' p)
+        (cbor_raw_get_header')
         ()
-        (ser_payload f p)
+        (ser_payload f)
       )
     )
     (Classical.forall_intro parse_raw_data_item_eq; serialize_raw_data_item)
 
 let ser_pre
-  (p: perm)
-  (x': cbor_raw)
+  (x': with_perm cbor_raw)
   (x: raw_data_item)
   (out: S.slice LP.byte)
   (offset: SZ.t)
   (v: Ghost.erased LP.bytes)
 : Tot slprop
 =
-    (S.pts_to out v ** cbor_match p x' x ** pure (
+    (S.pts_to out v ** cbor_match_with_perm x' x ** pure (
       SZ.v offset + Seq.length (bare_serialize serialize_raw_data_item x) <= Seq.length v
     ))
 
 let ser_post
-  (p: perm)
-  (x': cbor_raw)
+  (x': with_perm cbor_raw)
   (x: raw_data_item)
   (out: S.slice LP.byte)
   (offset: SZ.t)
@@ -346,7 +387,7 @@ let ser_post
 : Tot slprop
 =
   exists* v' .
-      S.pts_to out v' ** cbor_match p x' x ** pure (
+      S.pts_to out v' ** cbor_match_with_perm x' x ** pure (
       let bs = bare_serialize serialize_raw_data_item x in
       SZ.v res == SZ.v offset + Seq.length bs /\
       SZ.v res <= Seq.length v /\
@@ -358,15 +399,14 @@ let ser_post
 inline_for_extraction
 ```pulse
 fn ser_fold
-  (f: (p: perm) -> (x': cbor_raw) -> (x: Ghost.erased raw_data_item) -> (out: S.slice LP.byte) -> (offset: SZ.t) -> (v: Ghost.erased LP.bytes) -> stt SZ.t (ser_pre p x' x out offset v) (fun res -> ser_post p x' x out offset v res))
-  (p: perm)
-: LP.l2r_writer #cbor_raw #raw_data_item (cbor_match p) #parse_raw_data_item_kind #parse_raw_data_item serialize_raw_data_item
+  (f: (x': with_perm cbor_raw) -> (x: Ghost.erased raw_data_item) -> (out: S.slice LP.byte) -> (offset: SZ.t) -> (v: Ghost.erased LP.bytes) -> stt SZ.t (ser_pre x' x out offset v) (fun res -> ser_post x' x out offset v res))
+: LP.l2r_writer #_ #raw_data_item (cbor_match_with_perm) #parse_raw_data_item_kind #parse_raw_data_item serialize_raw_data_item
 =
-  (x': cbor_raw) (#x: raw_data_item) (out: S.slice LP.byte) (offset: SZ.t) (#v: Ghost.erased LP.bytes)
+  (x': with_perm cbor_raw) (#x: raw_data_item) (out: S.slice LP.byte) (offset: SZ.t) (#v: Ghost.erased LP.bytes)
 {
-  fold (ser_pre p x' x out offset v);
-  let res = f p x' x out offset v;
-  unfold (ser_post p x' x out offset v res);
+  fold (ser_pre x' x out offset v);
+  let res = f x' x out offset v;
+  unfold (ser_post x' x out offset v res);
   res
 }
 ```
@@ -374,22 +414,21 @@ fn ser_fold
 inline_for_extraction
 ```pulse
 fn ser_unfold
-  (f: (p: perm) -> LP.l2r_writer (cbor_match p) serialize_raw_data_item)
-  (p: perm)
-  (x': cbor_raw)
+  (f: LP.l2r_writer (cbor_match_with_perm) serialize_raw_data_item)
+  (x': with_perm cbor_raw)
   (x: Ghost.erased raw_data_item)
   (out: S.slice LP.byte)
   (offset: SZ.t)
   (v: Ghost.erased LP.bytes)
 requires
-  (ser_pre p x' x out offset v)
+  (ser_pre x' x out offset v)
 returns res: SZ.t
 ensures
-  (ser_post p x' x out offset v res)
+  (ser_post x' x out offset v res)
 {
-  unfold (ser_pre p x' x out offset v);
-  let res = f p x' out offset;
-  fold (ser_post p x' x out offset v res);
+  unfold (ser_pre x' x out offset v);
+  let res = f x' out offset;
+  fold (ser_post x' x out offset v res);
   res
 }
 ```
@@ -397,40 +436,40 @@ ensures
 inline_for_extraction
 ```pulse
 fn ser_body'
-  (f: (p: perm) -> (x': cbor_raw) -> (x: Ghost.erased raw_data_item) -> (out: S.slice LP.byte) -> (offset: SZ.t) -> (v: Ghost.erased LP.bytes) -> stt SZ.t (ser_pre p x' x out offset v) (fun res -> ser_post p x' x out offset v res))
-  (p: perm)
-  (x': cbor_raw)
+  (f: (x': with_perm cbor_raw) -> (x: Ghost.erased raw_data_item) -> (out: S.slice LP.byte) -> (offset: SZ.t) -> (v: Ghost.erased LP.bytes) -> stt SZ.t (ser_pre x' x out offset v) (fun res -> ser_post x' x out offset v res))
+  (x': with_perm cbor_raw)
   (x: Ghost.erased raw_data_item)
   (out: S.slice LP.byte)
   (offset: SZ.t)
   (v: Ghost.erased LP.bytes)
 requires
-  (ser_pre p x' x out offset v)
+  (ser_pre x' x out offset v)
 returns res: SZ.t
 ensures
-  ser_post p x' x out offset v res
+  ser_post x' x out offset v res
 {
-  ser_unfold (ser_fold f) p x' x out offset v;
+  ser_unfold (ser_fold f) x' x out offset v;
 }
 ```
 
-inline_for_extraction
 ```pulse
 fn rec ser'
-  (p: perm)
-  (x': cbor_raw)
+  (x': with_perm cbor_raw)
   (x: Ghost.erased raw_data_item)
   (out: S.slice LP.byte)
   (offset: SZ.t)
   (v: Ghost.erased LP.bytes)
 requires
-  (ser_pre p x' x out offset v)
+  (ser_pre x' x out offset v)
 returns res: SZ.t
 ensures
-  ser_post p x' x out offset v res
+  ser_post x' x out offset v res
 {
-  ser_body' ser' p x' x out offset v
+  ser_body' ser' x' x out offset v
 }
 ```
 
-let ser (p: perm) : l2r_writer (cbor_match p) serialize_raw_data_item = ser_fold ser' p
+let ser (p: perm) : l2r_writer (cbor_match p) serialize_raw_data_item =
+  l2r_writer_lens
+    (cbor_match_with_perm_lens p)
+    (ser_fold ser')
